% Generated by xcas
\documentclass{article} 
 \usepackage{pst-plot,color} 
 \begin{document} 
\begin{equation} \label{eq:0}
\mbox{\tt'restart'} = []
\end{equation}
\begin{verbatim}
 (x)->A*x^alpha
\end{verbatim}\begin{verbatim}
 (x)->(D( (x)->A*x^alpha))(x)
\end{verbatim}\begin{equation} \label{eq:3}
\mbox{cas\_setup}(0,0,0,1,0,     0.000000,12,1,0,0,0),\mbox{maple\_mode}(1) = 0,0,0,1,0,     0.000000,12,1,0,0,0,\mbox{Warning: some commands like subs might change arguments order}
\end{equation}
\begin{verbatim}
 (x)->A*alpha*x^alpha/x
\end{verbatim}\begin{verbatim}
 (x)->fp(x)-mu*x
\end{verbatim}\begin{verbatim}
 (x)->fp1(x)-mu
\end{verbatim}\begin{verbatim}
 (x)->ln(x)
\end{verbatim}\begin{verbatim}
 (` x`)->1/` x`
\end{verbatim}\begin{verbatim}
 (c,k,p)->Util(c)+p*(fpn(k)-c)
\end{verbatim}\begin{equation} \label{eq:10}
cn1:=\frac{\partial \left(Hamilton(c,k,p)\right)}{\partial c} = (c)^{-1}-p
\end{equation}
\begin{equation} \label{eq:11}
eqadj:=\frac{\partial \left(Hamilton(c,k,p)\right)}{\partial k} = p\* (\frac{A\* alpha}{k} \* k^{alpha}-mu)
\end{equation}
\begin{equation} \label{eq:12}
cn_1:=\mbox{expr}(\mbox{subs([c=(c(t)),p=(p(t))],cn1)},1) = (c)^{-1}-p
\end{equation}
\begin{equation} \label{eq:13}
cn_0:=\mbox{expr}(\mbox{subs([c=(c(t))],cn1)},1) = (c)^{-1}-p
\end{equation}
\begin{equation} \label{eq:14}
cn_1:=\mbox{expr}(\mbox{subs(c=(c(t)),p=(p(t)),cn1)},1) = (c(t))^{-1}-(p(t))
\end{equation}
\begin{equation} \label{eq:15}
eqadj_1:=\mbox{simplify}(\mbox{expr}(\mbox{subs(p=(p(t)),k=(k(t)),eqadj)},1)) = \frac{(p(t)\* A\* alpha\* (k(t))^{alpha}-(p(t)\* k(t)\* mu))}{k(t)}
\end{equation}
\begin{equation} \label{eq:16}
ed1:=\frac{\partial \left(p(t)\right)}{\partial t}-(\mbox{\tt'psi'}\* p(t))+eqadj_1 = \frac{\partial \left(p(t)\right)}{\partial t}-(\mbox{\tt'psi'}\* p(t))+\frac{(p(t)\* A\* alpha\* (k(t))^{alpha}-(p(t)\* k(t)\* mu))}{k(t)}
\end{equation}
\begin{equation} \label{eq:17}
\mbox{expr}(\mbox{subs(p(t)=(1/(c(t))),ed1)},1) = \frac{\partial \left((~c(t))^{-1}\right)}{\partial t}-(\frac{\mbox{\tt'psi'}}{c(t)})+\frac{(\frac{1}{c(t)} \* A\* alpha\* (k(t))^{alpha}-(\frac{1}{c(t)} \* k(t)\* mu))}{k(t)}
\end{equation}
\begin{equation} \label{eq:18}
ed1:=\mbox{ans()} = \frac{\partial \left((c(t))^{-1}\right)}{\partial t}-(\frac{\mbox{\tt'psi'}}{c(t)})+\frac{(\frac{1}{c(t)} \* A\* alpha\* (k(t))^{alpha}-(\frac{1}{c(t)} \* k(t)\* mu))}{k(t)}
\end{equation}
\begin{equation} \label{eq:19}
edc:=\mbox{simplify}((c(t))^{2}\* ed1) = \mbox{simplify Bad Argument Type}
\end{equation}
\begin{equation} \label{eq:20}
(c(t))^{2}\* ed1 = (c(t))^{2}\* (\frac{(-(\frac{\partial \left(c(t)\right)}{\partial t}))}{(c(t))^{2}}-(\frac{\mbox{\tt'psi'}}{c(t)})+\frac{(\frac{1}{c(t)} \* A\* alpha\* (k(t))^{alpha}-(\frac{1}{c(t)} \* k(t)\* mu))}{k(t)})
\end{equation}
\begin{equation} \label{eq:21}
\mbox{ans()} = (c(t))^{2}\* (\frac{(-(\frac{\partial \left(c(t)\right)}{\partial t}))}{(c(t))^{2}}-(\frac{\mbox{\tt'psi'}}{c(t)})+\frac{(\frac{1}{c(t)} \* A\* alpha\* (k(t))^{alpha}-(\frac{1}{c(t)} \* k(t)\* mu))}{k(~t)})
\end{equation}
simplify(%\\
\begin{equation} \label{eq:23}
~edc:=(c(t))^{2}\* ed1 = (c(t))^{2}\* (\frac{(-(\frac{\partial \left(c(t)\right)}{\partial t}))}{(c(t))^{2}}-(\frac{\mbox{\tt'psi'}}{c(t)})+\frac{(\frac{1}{c(t)} \* A\* alpha\* (k(t))^{alpha}-(\frac{1}{c(t)} \* k(t)\* mu))}{k(t)})
\end{equation}
\begin{equation} \label{eq:24}
\mbox{simplify}(edc) = \mbox{simplify Bad Argument Type}
\end{equation}
\begin{equation} \label{eq:25}
edk:=(\frac{\partial \left(k(t)\right)}{\partial t})=(fpn(k(t))-(c(t))) = (\frac{\partial \left(k(t)\right)}{\partial t})=(A\* (k(t))^{alpha}-(mu\* \mbox{of}([k,t]))-(c(t)))
\end{equation}
\begin{equation} \label{eq:26}
\mbox{expr}(\mbox{subs(diff(c(t),t)=0,edc)},1) = (c(t))^{2}\* (\frac{(-0)}{(c(t))^{2}}-(\frac{\mbox{\tt'psi'}}{c(t)})+\frac{(\frac{1}{c(t)} \* A\* alpha\* (k(t))^{alpha}-(\frac{1}{c(t)} \* k(t)\* mu))}{k(t)})
\end{equation}
subs(c(t)=c,k(t)=k,%\\
\begin{equation} \label{eq:28}
s1:=\mbox{expr}(\mbox{subs(diff(c(t),t)=0,edc)},1) = (c(t))^{2}\* (\frac{(-0)}{(c(t))^{2}}-(\frac{\mbox{\tt'psi'}}{c(t)})+\frac{(\frac{1}{c(t)} \* A\* alpha\* (k(t))^{alpha}-(\frac{1}{c(t)} \* k(t)\* mu))}{k(t)})
\end{equation}
\begin{equation} \label{eq:29}
s2:=\mbox{expr}(\mbox{subs(c(t)=c,k(t)=k,s1)},1) = c^{2}\* (-(\frac{\mbox{\tt'psi'}}{c})+\frac{(\frac{1}{c} \* A\* alpha\* k^{alpha}-(\frac{1}{c} \* k\* mu))}{k})
\end{equation}
\begin{equation} \label{eq:30}
eqc:=s2 = c^{2}\* (-(\frac{\mbox{\tt'psi'}}{c})+\frac{(\frac{1}{c} \* A\* alpha\* k^{alpha}-(\frac{1}{c} \* k\* mu))}{k})
\end{equation}
\begin{equation} \label{eq:31}
s3:=\mbox{expr}(\mbox{subs(c(t)=c,k(t)=k,rhs(edk))},1) = A\* k^{alpha}-(mu\* k)-c
\end{equation}
\begin{equation} \label{eq:32}
eqk:=s3 = A\* k^{alpha}-(mu\* k)-c
\end{equation}
\begin{equation} \label{eq:33}
eqk = A\* k^{alpha}-(mu\* k)-c
\end{equation}
\begin{equation} \label{eq:34}
A:=(     8.000000) =      8.000000
\end{equation}
\begin{equation} \label{eq:35}
alpha:=(     0.300000) =      0.300000
\end{equation}
\begin{equation} \label{eq:36}
mu:=(     0.100000) =      0.100000
\end{equation}
\begin{equation} \label{eq:37}
\mbox{\tt'psi'}:=(     0.050000) = [\mbox{'psi' is a reserved word, sto not allowed:},     0.050000]
\end{equation}

\end{document}
